Some fixes for functions, and added struct_unfold macro

concordium-provider/src/auction_provider.rs
@@ -1,7 +1,7 @@
-use concordium_std::{collections::BTreeMap, *};
-use core::fmt::Debug;
 use crate::provider::Action;
 use auction::*;
+use concordium_std::{collections::BTreeMap, *};
+use core::fmt::Debug;
 use hacspec_lib::*;
 
 /// # Implementation of an auction smart contract
@@ -44,93 +44,72 @@ pub struct State {
     auction_state: AuctionState,
     /// The highest bid so far (stored explicitly so that bidders can quickly
     /// see it)
-    highest_bid:   concordium_std::Amount,
+    highest_bid: concordium_std::Amount,
     /// The sold item (to be displayed to the auction participants), encoded in
     /// ASCII
-    item:          Vec<u8>,
+    item: Vec<u8>,
     /// Expiration time of the auction at which bids will be closed (to be
     /// displayed to the auction participants)
-    expiry:        concordium_std::Timestamp,
+    expiry: concordium_std::Timestamp,
     /// Keeping track of which account bid how much money
     #[concordium(size_length = 2)]
-    bids:          BTreeMap<AccountAddress, concordium_std::Amount>,
+    bids: BTreeMap<AccountAddress, concordium_std::Amount>,
 }
 
-fn user_address_to_accout_address (acc : UserAddress) -> AccountAddress {
-    AccountAddress (
-        [acc[0],
-	 acc[1],
-	 acc[2],
-	 acc[3],
-	 acc[4],
-	 acc[5],
-	 acc[6],
-	 acc[7],
-	 acc[8],
-	 acc[9],
-	 acc[10],
-	 acc[11],
-	 acc[12],
-	 acc[13],
-	 acc[14],
-	 acc[15],
-	 acc[16],
-	 acc[17],
-	 acc[18],
-	 acc[19],
-	 acc[20],
-	 acc[21],
-	 acc[22],
-	 acc[23],
-	 acc[24],
-	 acc[25],
-	 acc[26],
-	 acc[27],
-	 acc[28],
-	 acc[29],
-	 acc[30],
-	 acc[31],])
+fn user_address_to_accout_address(acc: UserAddress) -> AccountAddress {
+    AccountAddress([
+        acc[0], acc[1], acc[2], acc[3], acc[4], acc[5], acc[6], acc[7], acc[8], acc[9], acc[10],
+        acc[11], acc[12], acc[13], acc[14], acc[15], acc[16], acc[17], acc[18], acc[19], acc[20],
+        acc[21], acc[22], acc[23], acc[24], acc[25], acc[26], acc[27], acc[28], acc[29], acc[30],
+        acc[31],
+    ])
 }
 
-fn my_auction_state_to_their_auction_state(s : auction::AuctionState) -> AuctionState {
+fn my_auction_state_to_their_auction_state(s: auction::AuctionState) -> AuctionState {
     match s {
         auction::AuctionState::NotSoldYet => AuctionState::NotSoldYet,
-        auction::AuctionState::Sold (a) => AuctionState::Sold (user_address_to_accout_address(a)),
+        auction::AuctionState::Sold(a) => AuctionState::Sold(user_address_to_accout_address(a)),
     }
 }
 
+fn seq_map_to_btree_map(m: SeqMap) -> BTreeMap<AccountAddress, concordium_std::Amount> {
+    let m1prime =
+        (0..m.0.len() / 32).map(|x| UserAddress::from_seq(&m.0.clone().slice(x * 32, 32)));
+    let m2prime =
+        (0..m.1.len() / 8).map(|x| u64_from_be_bytes(u64Word::from_seq(&m.1.slice(x * 8, 8))));
 
-fn seq_map_to_btree_map (m : SeqMap) -> BTreeMap<AccountAddress, concordium_std::Amount> {
-    let (m1,m2) = m;
-
-    let m1prime = (0..m1.len() / 32).map(|x| UserAddress::from_seq(&m1.clone().slice(x * 32,32)));
-    let m2prime = (0..m2.len() / 8).map(|x| u64_from_be_bytes(u64Word::from_seq(&m2.slice(x * 8, 8))));
-
-    (m1prime.zip(m2prime)).fold(BTreeMap::new(), |mut t, (x, y)| { t.insert(user_address_to_accout_address (x), concordium_std::Amount { micro_gtu: y }); t } )
+    (m1prime.zip(m2prime)).fold(BTreeMap::new(), |mut t, (x, y)| {
+        t.insert(
+            user_address_to_accout_address(x),
+            concordium_std::Amount { micro_gtu: y },
+        );
+        t
+    })
 }
 
-
-fn my_state_to_their_state (s : auction::State) -> State {
-    let (a,b,c,d,e) = s;
+fn my_state_to_their_state(s: auction::State) -> State {
     State {
-        auction_state: my_auction_state_to_their_auction_state(a),
-        highest_bid: concordium_std::Amount { micro_gtu: b },
-        item: c.native_slice().to_vec(),
-        expiry: concordium_std::Timestamp::from_timestamp_millis(d),
-        bids: seq_map_to_btree_map(e),
+        auction_state: my_auction_state_to_their_auction_state(s.0),
+        highest_bid: concordium_std::Amount { micro_gtu: s.1 },
+        item: s.2.native_slice().to_vec(),
+        expiry: concordium_std::Timestamp::from_timestamp_millis(s.3),
+        bids: seq_map_to_btree_map(s.4),
     }
 }
 
 /// A helper function to create a state for a new auction.
 fn fresh_state(itm: Vec<u8>, exp: concordium_std::Timestamp) -> State {
-    my_state_to_their_state(auction::fresh_state(Seq::from_vec(itm), exp.timestamp_millis()))
+    my_state_to_their_state(auction::fresh_state(
+        Seq::from_vec(itm),
+        exp.timestamp_millis(),
+    ))
 }
 
 /// Type of the parameter to the `init` function.
 #[derive(Serialize, SchemaType)]
 pub struct InitParameter {
     /// The item to be sold, as a sequence of ASCII codes.
-    item:   Vec<u8>,
+    item: Vec<u8>,
     /// Time of the auction end in the RFC 3339 format (https://tools.ietf.org/html/rfc3339)
     expiry: concordium_std::Timestamp,
 }
@@ -162,71 +141,65 @@ pub fn auction_init(ctx: &impl HasInitContext) -> InitResult<State> {
     Ok(fresh_state(parameter.item, parameter.expiry))
 }
 
-fn u8x32_to_user_address (acc : [u8;32]) -> UserAddress {
-    UserAddress ([acc[0],
-		  acc[1],
-		  acc[2],
-		  acc[3],
-		  acc[4],
-		  acc[5],
-		  acc[6],
-		  acc[7],
-		  acc[8],
-		  acc[9],
-		  acc[10],
-		  acc[11],
-		  acc[12],
-		  acc[13],
-		  acc[14],
-		  acc[15],
-		  acc[16],
-		  acc[17],
-		  acc[18],
-		  acc[19],
-		  acc[20],
-		  acc[21],
-		  acc[22],
-		  acc[23],
-		  acc[24],
-		  acc[25],
-		  acc[26],
-		  acc[27],
-		  acc[28],
-		  acc[29],
-		  acc[30],
-		  acc[31],])
+fn u8x32_to_user_address(acc: [u8; 32]) -> UserAddress {
+    UserAddress([
+        acc[0], acc[1], acc[2], acc[3], acc[4], acc[5], acc[6], acc[7], acc[8], acc[9], acc[10],
+        acc[11], acc[12], acc[13], acc[14], acc[15], acc[16], acc[17], acc[18], acc[19], acc[20],
+        acc[21], acc[22], acc[23], acc[24], acc[25], acc[26], acc[27], acc[28], acc[29], acc[30],
+        acc[31],
+    ])
 }
 
-fn their_auction_state_to_my_auction_state (s : AuctionState) -> auction::AuctionState {
+fn their_auction_state_to_my_auction_state(s: AuctionState) -> auction::AuctionState {
     match s {
         AuctionState::NotSoldYet => auction::AuctionState::NotSoldYet,
-        AuctionState::Sold (a) => auction::AuctionState::Sold (u8x32_to_user_address(a.0)),
+        AuctionState::Sold(a) => auction::AuctionState::Sold(u8x32_to_user_address(a.0)),
     }
 }
 
-fn btree_map_to_seq_map (m : BTreeMap<AccountAddress, concordium_std::Amount>) -> SeqMap {
-    (m.keys().map(|x| u8x32_to_user_address(x.0)).fold(PublicByteSeq::new(0_usize), |v,x| v.concat(&x)),
-     m.values().map(|x| x.micro_gtu).fold(PublicSeq::new(0_usize), |v, x| v.concat(&u64_to_be_bytes(x))))
+fn btree_map_to_seq_map(m: BTreeMap<AccountAddress, concordium_std::Amount>) -> SeqMap {
+    SeqMap(
+        m.keys()
+            .map(|x| u8x32_to_user_address(x.0))
+            .fold(PublicByteSeq::new(0_usize), |v, x| v.concat(&x)),
+        m.values()
+            .map(|x| x.micro_gtu)
+            .fold(PublicSeq::new(0_usize), |v, x| {
+                v.concat(&u64_to_be_bytes(x))
+            }),
+    )
 
     // Seq::from_vec(m.keys().map(|x| u8x32_to_user_address(x.0)).zip(m.values().map(|(x)| x.micro_gtu)).collect())
 }
 
-fn their_state_to_my_state (s : &mut State) -> auction::State {
-(their_auction_state_to_my_auction_state(s.auction_state.clone()),s.highest_bid.micro_gtu,Seq::from_vec(s.item.clone()),s.expiry.timestamp_millis(),btree_map_to_seq_map(s.bids.clone()))
+fn their_state_to_my_state(s: &mut State) -> auction::State {
+    State (
+        their_auction_state_to_my_auction_state(s.auction_state.clone()),
+        s.highest_bid.micro_gtu,
+        Seq::from_vec(s.item.clone()),
+        s.expiry.timestamp_millis(),
+        btree_map_to_seq_map(s.bids.clone()),
+    )
 }
 
-fn their_context_to_my_context (ctx: &impl HasReceiveContext) -> auction::Context {
-    (ctx.metadata().slot_time().timestamp_millis(),
-     match ctx.sender() {
-         Address::Contract(_) => UserAddressSet::UserAddressNone,
-         Address::Account(account_address) => UserAddressSet::UserAddressSome (u8x32_to_user_address(account_address.0), ()),
-     })
+fn their_context_to_my_context(ctx: &impl HasReceiveContext) -> auction::Context {
+    (
+        ctx.metadata().slot_time().timestamp_millis(),
+        match ctx.sender() {
+            Address::Contract(_) => UserAddressSet::UserAddressNone,
+            Address::Account(account_address) => {
+                UserAddressSet::UserAddressSome(u8x32_to_user_address(account_address.0), ())
+            }
+        },
+    )
 }
 
-fn their_context_to_my_finalize_context (ctx: &impl HasReceiveContext) -> auction::FinalizeContext {
-    (ctx.metadata().slot_time().timestamp_millis(),
-     u8x32_to_user_address(ctx.owner().0),
-     ctx.self_balance().micro_gtu)
+fn their_context_to_my_finalize_context(ctx: &impl HasReceiveContext) -> auction::FinalizeContext {
+    (
+        ctx.metadata().slot_time().timestamp_millis(),
+        u8x32_to_user_address(ctx.owner().0),
+        ctx.self_balance().micro_gtu,
+    )
 }
 
 /// Receive function in which accounts can bid before the auction end time
@@ -236,15 +209,21 @@ pub fn auction_bid<A: HasActions>(
     amount: concordium_std::Amount,
     state: &mut State,
 ) -> Result<A, BidError> {
-    let (new_state, res) = auction::auction_bid(their_context_to_my_context(ctx), amount.micro_gtu, their_state_to_my_state(state));
+    let (new_state, res) = auction::auction_bid(
+        their_context_to_my_context(ctx),
+        amount.micro_gtu,
+        their_state_to_my_state(state),
+    );
     *state = my_state_to_their_state(new_state);
-    
+
     match res {
         Ok(_) => Ok(A::accept()),
-        Err(auction::BidError::ContractSender) =>                        Err(BidError::ContractSender),
-        Err(auction::BidError::BidTooLow) =>                             Err(BidError::BidTooLow),
-        Err(auction::BidError::BidsOverWaitingForAuctionFinalization) => Err(BidError::BidsOverWaitingForAuctionFinalization),
-        Err(auction::BidError::AuctionIsFinalized) =>                    Err(BidError::AuctionFinalized),
+        Err(auction::BidError::ContractSender) => Err(BidError::ContractSender),
+        Err(auction::BidError::BidTooLow) => Err(BidError::BidTooLow),
+        Err(auction::BidError::BidsOverWaitingForAuctionFinalization) => {
+            Err(BidError::BidsOverWaitingForAuctionFinalization)
+        }
+        Err(auction::BidError::AuctionIsFinalized) => Err(BidError::AuctionFinalized),
     }
 }
 
@@ -255,22 +234,50 @@ pub fn auction_finalize<A: HasActions>(
     ctx: &impl HasReceiveContext,
     state: &mut State,
 ) -> Result<A, FinalizeError> {
-    let (new_state, res) = auction::auction_finalize(their_context_to_my_finalize_context(ctx), their_state_to_my_state(state));
+    let (new_state, res) = auction::auction_finalize(
+        their_context_to_my_finalize_context(ctx),
+        their_state_to_my_state(state),
+    );
     *state = my_state_to_their_state(new_state);
-    
+
     match res {
-        Ok(FinalizeAction::Accept) => {println!("ACCEPT"); Ok(A::accept())},
-        Ok(FinalizeAction::SimpleTransfer(owner, b, s)) =>
-            {println!("Simple Transfer"); 
-            Ok((0..s.len() / (32+8))
-               .fold(A::simple_transfer(&user_address_to_accout_address(owner), concordium_std::Amount { micro_gtu: b }),
-                     |t,x| t.and_then(A::simple_transfer(
-                         &user_address_to_accout_address(UserAddress::from_seq(&s.slice(x * (32+8), 32))),
-                         concordium_std::Amount { micro_gtu: u64_from_be_bytes(u64Word::from_seq(&s.slice(x * (32+8) + 32,8))) })
-                     )))},
-        Err(auction::FinalizeError::BidMapError) => {println!("Bid map error"); Err(FinalizeError::BidMapError)},
-        Err(auction::FinalizeError::AuctionStillActive) => {println!("Auction still alive"); Err(FinalizeError::AuctionStillActive)},
-        Err(auction::FinalizeError::AuctionFinalized) => {println!("Auction finalized"); Err(FinalizeError::AuctionFinalized)},
+        Ok(FinalizeAction::Accept) => {
+            println!("ACCEPT");
+            Ok(A::accept())
+        }
+        Ok(FinalizeAction::SimpleTransfer(owner, b, s)) => {
+            println!("Simple Transfer");
+            Ok((0..s.len() / (32 + 8)).fold(
+                A::simple_transfer(
+                    &user_address_to_accout_address(owner),
+                    concordium_std::Amount { micro_gtu: b },
+                ),
+                |t, x| {
+                    t.and_then(A::simple_transfer(
+                        &user_address_to_accout_address(UserAddress::from_seq(
+                            &s.slice(x * (32 + 8), 32),
+                        )),
+                        concordium_std::Amount {
+                            micro_gtu: u64_from_be_bytes(u64Word::from_seq(
+                                &s.slice(x * (32 + 8) + 32, 8),
+                            )),
+                        },
+                    ))
+                },
+            ))
+        }
+        Err(auction::FinalizeError::BidMapError) => {
+            println!("Bid map error");
+            Err(FinalizeError::BidMapError)
+        }
+        Err(auction::FinalizeError::AuctionStillActive) => {
+            println!("Auction still alive");
+            Err(FinalizeError::AuctionStillActive)
+        }
+        Err(auction::FinalizeError::AuctionFinalized) => {
+            println!("Auction finalized");
+            Err(FinalizeError::AuctionFinalized)
+        }
     }
 }
 
@@ -279,9 +286,14 @@ pub fn auction_finalize<A: HasActions>(
 const AUCTION_END: u64 = 1;
 const ITEM: &str = "Starry night by Van Gogh";
 
-pub fn dummy_fresh_state() -> State { dummy_active_state(concordium_std::Amount::zero(), BTreeMap::new()) }
+pub fn dummy_fresh_state() -> State {
+    dummy_active_state(concordium_std::Amount::zero(), BTreeMap::new())
+}
 
-pub fn dummy_active_state(highest: concordium_std::Amount, bids: BTreeMap<AccountAddress, concordium_std::Amount>) -> State {
+pub fn dummy_active_state(
+    highest: concordium_std::Amount,
+    bids: BTreeMap<AccountAddress, concordium_std::Amount>,
+) -> State {
     // State {
     //     auction_state: my_auction_state_to_their_auction_state(a),
     //     highest_bid: Amount { micro_gtu: b },
@@ -289,7 +301,7 @@ pub fn dummy_active_state(highest: concordium_std::Amount, bids: BTreeMap<Accoun
     //     expiry: Timestamp::from_timestamp_millis(d),
     //     bids: seq_map_to_btree_map(e),
     // }
-    
+
     State {
         auction_state: AuctionState::NotSoldYet,
         highest_bid: highest,
@@ -299,12 +311,13 @@ pub fn dummy_active_state(highest: concordium_std::Amount, bids: BTreeMap<Accoun
     }
 }
 
-pub fn make_state (
+pub fn make_state(
     auction_state: AuctionState,
-    highest_bid:   concordium_std::Amount,
-    item:          Vec<u8>,
-    expiry:        concordium_std::Timestamp,
-    bids:          BTreeMap<AccountAddress, concordium_std::Amount>) -> State {
+    highest_bid: concordium_std::Amount,
+    item: Vec<u8>,
+    expiry: concordium_std::Timestamp,
+    bids: BTreeMap<AccountAddress, concordium_std::Amount>,
+) -> State {
     State {
         auction_state: auction_state,
         highest_bid: highest_bid,
@@ -319,12 +332,12 @@ pub fn make_state (
 //     highest_bid:   winning_amount,
 //     item:          ITEM.as_bytes().to_vec(),
 //     expiry:        Timestamp::from_timestamp_millis(AUCTION_END),
-//     bids:          bid_map,    
+//     bids:          bid_map,
 // }
 
 pub fn item_expiry_parameter() -> InitParameter {
     InitParameter {
-        item:   ITEM.as_bytes().to_vec(),
+        item: ITEM.as_bytes().to_vec(),
         expiry: concordium_std::Timestamp::from_timestamp_millis(AUCTION_END),
     }
 }
