lib/src/struct_unfold.rs
@@ -1,0 +1,16 @@
+#[macro_export]
+macro_rules! unfold_struct {
+    (
+     struct $struct_name:ident {
+        $(
+        $field_name:ident : $field_type:ty
+        ),*$(,)+
+    }
+    ) => {
+            pub type $struct_name = (
+                $(
+                    $field_type
+                ),*
+            );
+    }
+}
